Make the interpreter for constant time programs provable.
This involves removing references the somewhat fancy monadic construct.
Passing around the direction list using the bind construct makes Coq
forget the relation between the different variables, resulting in an
impossible proof.

TestingSpecCT.v
@@ -1293,33 +1293,35 @@ Inductive spec_eval : com -> state -> astate -> bool -> dirs ->
 (* We're forced to change `spec_eval` quite a bit, because for the sequence,
    we cannot simply guess the two `ds`. Instead, return the elements of `ds` we didn't consume. *)
 Inductive eval_return_type : Type :=
-  | RBlewUp : eval_return_type (* the execution blew up (by itself, without speculation) *)
-  | RInvalidDirection : eval_return_type (* the directions provided did not make sense *)
+  (* ran out of fuel *)
+  | ROutOfFuel : eval_return_type
+  (* the execution blew up (by itself, without speculation) *)
+  | RBlewUp : eval_return_type
+  (* the directions provided did not make sense *)
+  | RInvalidDirection : eval_return_type
   | ROk : state -> astate -> bool -> obs -> dirs -> eval_return_type.
-Definition ok_and (ret : eval_return_type) (f : state -> astate -> bool -> obs -> dirs -> eval_return_type) : eval_return_type :=
-  match ret with
-  | ROk st ast b os ds => f st ast b os ds
-  | _ => ret
-  end.
 
 (* Now with supports for loops. However, the length of ds and/or the size of the program will be strictly decreasing:
    no need for fuel. *)
-Fixpoint program_size (c : com) : nat := match c with
-  | <{ c1 ; c2 }> => S ((program_size c1) + (program_size c2))
-  | <{ if be then ct else cf end }> => S ((program_size ct) + (program_size cf))
-  | <{ while be do c end }> => S (program_size c)
-  | _ => 1
-  end.
-Program Fixpoint spec_eval_engine_aux (c : com) (st : state) (ast : astate) (b : bool) (ds : dirs) {measure ((Datatypes.length ds) + (program_size c))}: eval_return_type :=
+Fixpoint spec_eval_engine_aux (c : com) (st : state) (ast : astate) (b : bool) (ds : dirs) (f : nat): eval_return_type :=
+  match f with
+  | 0 => ROutOfFuel
+  | S f' =>
+
   match c with
   | <{ skip }> => ROk st ast b [] ds
   | <{ x := e }> => let n := aeval st e in
       ROk (x !-> n; st) ast b [] ds
   | <{ c1 ; c2 }> =>
-      ok_and (spec_eval_engine_aux c1 st ast b ds) (fun st' ast' b' os1 ds' =>
-      ok_and (spec_eval_engine_aux c2 st' ast' b' ds') (fun st'' ast'' b'' os2 ds'' =>
-        ROk st'' ast'' b'' (os1 ++ os2) ds''
-      ))
+      match spec_eval_engine_aux c1 st ast b ds f' with
+      | ROk st' ast' b' os1 ds' =>
+          match spec_eval_engine_aux c2 st' ast' b' ds' f' with
+          | ROk st'' ast'' b'' os2 ds'' =>
+              ROk st'' ast'' b'' (os1 ++ os2) ds''
+          | ret => ret
+          end
+      | ret => ret
+      end
   | <{ if be then ct else cf end }> =>
       match ds with
       | DStep::ds' =>
@@ -1328,18 +1330,22 @@ Program Fixpoint spec_eval_engine_aux (c : com) (st : state) (ast : astate) (b :
             (* normal execution... *)
             if condition then ct else cf in
 
-          ok_and (spec_eval_engine_aux next_c st ast b ds') (fun st' ast' b' os' ds'' =>
-            ROk st' ast' b' ((OBranch condition) :: os') ds''
-          )
+          match spec_eval_engine_aux next_c st ast b ds' f' with
+          | ROk st' ast' b' os' ds'' =>
+              ROk st' ast' b' ((OBranch condition) :: os') ds''
+          | ret => ret
+          end
       | DForce::ds' =>
           let condition := beval st be in
           let next_c :=
             (* branches swapped! *)
             if condition then cf else ct in
 
-          ok_and (spec_eval_engine_aux next_c st ast true ds') (fun st' ast' b' os' ds'' =>
-            ROk st' ast' b' ((OBranch condition) :: os') ds''
-          )
+          match spec_eval_engine_aux next_c st ast true ds' f' with
+          | ROk st' ast' b' os' ds'' =>
+              ROk st' ast' b' ((OBranch condition) :: os') ds''
+          | ret => ret
+          end
       | _ => RInvalidDirection
       end
   | <{ while be do c end }> =>
@@ -1348,20 +1354,30 @@ Program Fixpoint spec_eval_engine_aux (c : com) (st : state) (ast : astate) (b :
           let condition := beval st be in
 
           if condition then
-            ok_and (spec_eval_engine_aux c st ast b ds') (fun st' ast' b' os1 ds' =>
-            ok_and (spec_eval_engine_aux <{ while be do c end }> st' ast' b' ds') (fun st' ast' b' os2 ds' =>
-              ROk st' ast' b' (os1 ++ os2) ds'
-            ))
+            match spec_eval_engine_aux c st ast b ds' f' with
+            | ROk st' ast' b' os1 ds' =>
+                match spec_eval_engine_aux <{ while be do c end }> st' ast' b' ds' f' with
+                | ROk st' ast' b' os2 ds' => 
+                    ROk st' ast' b' (os1 ++ os2) ds'
+                | ret => ret
+                end
+            | ret => ret
+            end
           else
             ROk st ast b [OBranch condition] ds'
       | DForce::ds' =>
           let condition := beval st be in
 
           if negb condition then
-            ok_and (spec_eval_engine_aux c st ast true ds') (fun st' ast' b' os1 ds' =>
-            ok_and (spec_eval_engine_aux <{ while be do c end }> st' ast' b' ds') (fun st' ast' b' os2 ds' =>
-              ROk st' ast' b' (os1 ++ os2) ds'
-            ))
+            match spec_eval_engine_aux c st ast true ds' f' with
+            | ROk st' ast' b' os1 ds' =>
+                match spec_eval_engine_aux <{ while be do c end }> st' ast' b' ds' f' with
+                | ROk st' ast' b' os2 ds' =>
+                    ROk st' ast' b' (os1 ++ os2) ds'
+                | ret => ret
+                end
+            | ret => ret
+            end
           else
             ROk st ast b [OBranch condition] ds'
       | _ => RInvalidDirection
@@ -1425,55 +1441,34 @@ Program Fixpoint spec_eval_engine_aux (c : com) (st : state) (ast : astate) (b :
             RInvalidDirection
     | _ => RInvalidDirection
     end
+  end
   end.
-(* We must prove that the measure given is indeed strictly decreasing
-   TODO: this is hard because the use of ok_and makes Coq forget about relations between variables *)
-Next Obligation.
-  Admitted.
-Next Obligation.
-  Admitted.
-Next Obligation.
-  Admitted.
-Next Obligation.
-  Admitted.
-Next Obligation.
-  Admitted.
-Next Obligation.
-  Admitted.
-Next Obligation.
-  Admitted.
-Next Obligation.
-  Admitted.
-Next Obligation.
-  Admitted.
-Next Obligation.
-  Admitted.
-Next Obligation.
-  Admitted.
-Next Obligation.
-  Admitted.
-Next Obligation.
-  Admitted.
-Next Obligation.
-  Admitted.
-Next Obligation.
-  Admitted.
-Next Obligation.
-  Admitted.
-Next Obligation.
-  Admitted.
-Next Obligation.
-  Admitted.
-Next Obligation.
-  Admitted.
-Next Obligation.
-  Admitted.
-Definition spec_eval_engine (c : com) (st : state) (ast : astate) (b : bool) (ds : dirs) : option (state * astate * bool * obs) :=
-  match spec_eval_engine_aux c st ast b ds with
-  | ROk st' ast' b' os' [] =>
-      Some (st', ast', b', os')
-  | _ => None
+Fixpoint program_size (c : com) : nat :=
+  match c with
+  | <{ if be then c1 else c2 end }> => S ((program_size c1) + (program_size c2))
+  | <{ c1 ; c2 }> => S ((program_size c1) + (program_size c2))
+  | <{ while be do c end }> => S (program_size c)
+  | _ => 1
   end.
+Definition compute_gas (c : com) (ds : dirs) : nat :=
+  (S (Datatypes.length ds)) * (program_size c).
+Definition spec_eval_engine (c : com) (st : state) (ast : astate) (b : bool) (ds : dirs) : eval_return_type :=
+  spec_eval_engine_aux c st ast b ds (S (compute_gas c ds)).
+
+Theorem more_gas :
+  forall c st ast b ds f,
+    f > (compute_gas c ds) -> spec_eval_engine_aux c st ast b ds f <> ROutOfFuel.
+Proof.
+Admitted.
+
+Theorem enough_gas :
+  forall c st ast b ds, spec_eval_engine c st ast b ds <> ROutOfFuel.
+Proof.
+  intros c st ast b ds.
+  unfold spec_eval_engine.
+  apply more_gas.
+  apply Nat.lt_succ_diag_r.
+Qed.
 
 (* Simple tests *)
 Eval compute in
